trying to prove fixpoint: failed

proof/CorrectRel.v
@@ -1,4 +1,4 @@
-From bpf.src Require Import DxIntegers DxValues DxMemRegion DxRegs DxState DxMonad DxFlag.
+From bpf.src Require Import DxIntegers DxValues DxOpcode DxMemRegion DxRegs DxState DxMonad DxFlag.
 From Coq Require Import List Lia ZArith.
 From compcert Require Import Integers Values Clight Memory AST.
 Import ListNotations.
@@ -19,6 +19,11 @@ Definition valu32_correct (x:valu32_t) (v: val) :=
 Definition sint32_correct (x: sint32_t) (v: val) :=
   Vint x = v.
 
+Definition int8_correct (x: int8_t) (v: val) :=
+  Vint (Int.repr (Byte.unsigned x)) = v.
+
+Definition nat_correct (x: nat) (v: val) :=
+  Vint (Int.repr (Z.of_nat x)) = v.
 
 Definition reg_correct (r: reg) (v: val) :=
   (*complu_lt_32 v (Vint (Int.repr 11)) = true /\ (**r ensured by verifier *) *)
@@ -28,7 +33,11 @@ Definition reg_int64_correct (x:int64_t) (v: val) :=
   Vlong x = v /\
     0 <= (Int64.unsigned (Int64.shru (Int64.and x (Int64.repr 4095)) (Int64.repr 8))) <= 10.
 
-
+Definition opcode_mem_ld_imm_correct (opcode: opcode_mem_ld_imm) (v: val) :=
+  match opcode with
+  | op_BPF_LDDW => exists vi, v = Vint vi (**this one is too weak, but for current proof, it is enough *)
+  | op_BPF_LDX_IMM_ILLEGAL_INS => exists vi, v = Vint vi (*v = Vundef*)
+  end.
 
 Definition match_chunk (x : memory_chunk) (b: val) :=
   b = Vint (
