benchmark/correct_calc_sum.v
@@ -1,0 +1,159 @@
+From bpf.src Require Import DxIntegers DxValues DxMemRegion DxState DxMonad DxInstructions.
+From Coq Require Import List Lia.
+From compcert Require Import Integers Values Clight Memory.
+Import ListNotations.
+Require Import ZArith.
+
+From bpf.proof Require Import Clightlogic MatchState CorrectRel CommonLemma.
+
+From bpf.benchmark Require Import clightlogicexample BenchmarkTests.
+
+(**
+unsigned int calc_sum(unsigned int v, unsigned int n)
+{
+  unsigned int n1;
+  unsigned int nv;
+  if (n == 0U) {
+    return 0U;
+  } else {
+    n1 = n - 1U;
+    nv = get_add(v, 1U);
+    return calc_sum(nv, n1);
+  }
+}
+
+Print calc_sum.
+calc_sum = 
+fix calc_sum (v : valu32_t) (n : nat) {struct n} : M valu32_t :=
+  match n with
+  | 0 => returnM val32_zero
+  | S n1 => bindM (get_add v val32_one) (fun nv : valu32_t => calc_sum nv n1)
+  end
+     : valu32_t -> nat -> M valu32_t
+
+*)
+
+Section Calc_sum.
+
+  (** The program contains our function of interest [fn] *)
+  Definition p : Clight.program := prog.
+
+  (* [Args,Res] provides the mapping between the Coq and the C types *)
+  (* Definition Args : list CompilableType := [stateCompilableType].*)
+  Definition args : list Type := [(valu32_t:Type); (nat:Type)].
+  Definition res : Type := (valu32_t:Type).
+
+  (* [f] is a Coq Monadic function with the right type *)
+  Definition f : arrow_type args (M res) := calc_sum.
+
+  Variable state_block: block. (**r a block storing all rbpf state information? *)
+
+  (* [fn] is the Cligth function which has the same behaviour as [f] *)
+  Definition fn: Clight.function := f_calc_sum.
+
+  (* [match_arg] relates the Coq arguments and the C arguments *)
+  Definition match_arg_list : DList.t (fun x => x -> val -> stateM -> Memory.Mem.mem -> Prop) args :=
+    (DList.DCons (stateless valu32_correct)
+       (DList.DCons (stateless nat_correct)
+                    (DList.DNil _))).
+
+  (* [match_res] relates the Coq result and the C result *)
+  Definition match_res : res -> val -> stateM -> Memory.Mem.mem -> Prop := fun x v st m => valu32_correct x v.
+
+  Instance correct_function3_calc_sum : correct_function3 p args res f fn (nil) true match_arg_list match_res.
+  Proof.
+    correct_function_from_body.
+    correct_body.
+    (** should we induction c0 before correct_body *)
+    unfold INV.
+    unfold f.
+    repeat intro.
+    get_invariant_more _v.
+    get_invariant_more _n.
+
+    unfold stateless, valu32_correct in H0.
+    unfold stateless, nat_correct in H2.
+    destruct H0 as (Hc_eq & (vi & Hvi_eq)).
+    subst c v.
+    simpl in c0.
+    (*generalize c0.*)
+    induction c0.
+    {
+      simpl.
+      intros.
+      eexists. exists m, Events.E0.
+      repeat split; unfold step2.
+      -
+        apply Smallstep.plus_star.
+        eapply Smallstep.plus_left'; eauto.
+        eapply step_ifthenelse.
+        econstructor; eauto.
+        econstructor; eauto.
+        Transparent Archi.ptr64.
+        econstructor; eauto.
+        simpl.
+        unfold Cop.sem_cmp, Cop.sem_binarith, Cop.sem_cast; simpl.
+        rewrite <- H2. simpl.
+        reflexivity.
+        reflexivity.
+
+        rewrite Int_eq_one_zero.
+        unfold negb.
+
+        forward_plus.
+        econstructor; eauto.
+        reflexivity.
+        reflexivity.
+        reflexivity.
+
+      - eexists.
+        unfold val32_zero; reflexivity.
+      - constructor.
+        reflexivity.
+    }
+
+    simpl; simpl in IHc0.
+    unfold match_temp_env in H, IHc0.
+    
+    (**r
+      H2 :         Vint (Int.repr (Z.of_nat (S c0))) = v0
+      Ihc0: ... -> Vint (Int.repr (Z.of_nat c0)) = v0 -> ...
+    *)
+
+    (**according to the c function:
+unsigned int get_add(unsigned int x, unsigned int y)
+{
+  return x + y;
+}
+       1. return value should be  x+y
+       2. the memory is same
+      *)
+    destruct (calc_sum _ _ _) eqn: Heq; [idtac | apply I].
+    unfold calc_sum in Heq.
+    eexists. exists m, Events.E0.
+
+    repeat split; unfold step2.
+    -
+      apply Smallstep.plus_star.
+      (** TODO: adding Sreturn  more info by Ltac2 *)
+      eapply Smallstep.plus_one; eauto.
+      eapply step_return_1.
+      +
+        repeat econstructor; eauto.
+        Transparent Archi.ptr64.
+        unfold Cop.sem_binary_operation.
+        unfold Cop.sem_add, Cop.classify_add, Ctypes.typeconv; simpl.
+        unfold Cop.sem_binarith, Cop.sem_cast, Cop.classify_cast; simpl.
+        reflexivity.
+      + econstructor; eauto.
+      + reflexivity.
+    - simpl.
+      exists (Int.add vi vj); reflexivity.
+    - simpl.
+      constructor.
+      reflexivity.
+  Qed.
+
+End Calc_sum.
+
+Existing Instance correct_function3_calc_sum.
