benchmark/correct_get_opcode_mem_ld_imm.v
@@ -1,0 +1,104 @@
+From bpf.src Require Import DxIntegers DxValues DxOpcode DxMemRegion DxState DxMonad DxInstructions.
+From Coq Require Import List Lia.
+From compcert Require Import Integers Values Clight Memory.
+Import ListNotations.
+Require Import ZArith.
+
+From bpf.proof Require Import Clightlogic MatchState CorrectRel CommonLemma.
+
+From bpf.benchmark Require Import clightlogicexample.
+
+(**
+unsigned char get_opcode_mem_ld_imm(unsigned char op)
+{
+  return (unsigned char) (op & 255);
+}
+
+Print get_opcode_mem_ld_imm.
+get_opcode_mem_ld_imm = 
+fun op : int8_t => returnM (DxOpcode.byte_to_opcode_mem_ld_imm op)
+     : int8_t -> M DxOpcode.opcode_mem_ld_imm
+
+*)
+
+Section Get_opcode_mem_ld_imm.
+
+  (** The program contains our function of interest [fn] *)
+  Definition p : Clight.program := prog.
+
+  (* [Args,Res] provides the mapping between the Coq and the C types *)
+  (* Definition Args : list CompilableType := [stateCompilableType].*)
+  Definition args : list Type := [(int8_t:Type)].
+  Definition res : Type := (opcode_mem_ld_imm:Type).
+
+  (* [f] is a Coq Monadic function with the right type *)
+  Definition f : arrow_type args (M res) := get_opcode_mem_ld_imm.
+
+  Variable state_block: block. (**r a block storing all rbpf state information? *)
+
+  (* [fn] is the Cligth function which has the same behaviour as [f] *)
+  Definition fn: Clight.function := f_get_opcode_mem_ld_imm.
+
+  (* [match_arg] relates the Coq arguments and the C arguments *)
+  Definition match_arg_list : DList.t (fun x => x -> val -> stateM -> Memory.Mem.mem -> Prop) args :=
+    (DList.DCons (stateless int8_correct)
+                  (DList.DNil _)).
+
+  (* [match_res] relates the Coq result and the C result *)
+  Definition match_res : res -> val -> stateM -> Memory.Mem.mem -> Prop := fun x v st m => opcode_mem_ld_imm_correct x v.
+
+  Instance correct_function3_get_opcode_mem_ld_imm : correct_function3 p args res f fn (nil) true match_arg_list match_res.
+  Proof.
+    correct_function_from_body.
+    correct_body.
+    (** how to use correct_* *)
+    unfold INV.
+    unfold f.
+    repeat intro.
+    get_invariant_more _op.
+
+    unfold stateless, int8_correct in H1.
+    subst v.
+
+    (**according to the c function:
+unsigned char get_opcode_mem_ld_imm(unsigned char op)
+{
+  return (unsigned char) (op & 255);
+}
+      *)
+    eexists. exists m, Events.E0.
+
+    repeat split; unfold step2.
+    -
+      apply Smallstep.plus_star.
+      (** TODO: adding Sreturn  more info by Ltac2 *)
+      eapply Smallstep.plus_one; eauto.
+      eapply step_return_1.
+      +
+        repeat econstructor; eauto.
+        Transparent Archi.ptr64.
+        unfold Cop.sem_binary_operation.
+        unfold Cop.sem_and; simpl.
+        unfold Cop.sem_binarith, Cop.sem_cast, Cop.classify_cast; simpl.
+        reflexivity.
+        
+        reflexivity. 
+      + econstructor; eauto.
+      + reflexivity.
+    - simpl.
+      unfold match_res, byte_to_opcode_mem_ld_imm, opcode_mem_ld_imm_correct.
+      unfold int8_0xff.
+      destruct (match Byte.unsigned (Byte.and c (Byte.repr 255)) with
+  | 24%Z => op_BPF_LDDW
+  | _ => op_BPF_LDX_IMM_ILLEGAL_INS
+  end) eqn: Heq; eexists; reflexivity.
+    - simpl.
+      constructor.
+      simpl.
+      apply Int.zero_ext_idem.
+      lia.
+  Qed.
+
+End Get_opcode_mem_ld_imm.
+
+Existing Instance correct_function3_get_opcode_mem_ld_imm.
